nola/iris/inv.v
@@ -1,6 +1,5 @@
 (** * Nola later-free invariant *)
 
-From nola.util Require Export sem.
 From nola.bi Require Export updw.
 From nola.bi Require Import wpw.
 From nola.iris Require Export iprop.
@@ -8,7 +7,7 @@ From nola.iris Require Import sinv.
 From iris.base_logic.lib Require Export wsat invariants.
 From iris.algebra Require Import gset.
 From iris.proofmode Require Import proofmode.
-Import SemNotation iPropAppNotation UpdwNotation WpwNotation.
+Import iPropAppNotation UpdwNotation WpwNotation.
 
 Implicit Type (FML : oFunctor) (i : positive) (N : namespace).
 
@@ -50,9 +49,13 @@ Section inv.
   Local Definition inv_sem (sm : FML $oi Σ → iProp Σ) i Px : iProp Σ :=
     sm Px ∗ ownD {[i]} ∨ ownE {[i]}.
   (** [inv_sem sm] is non-expansive when [sm] is *)
-  Local Instance inv_sem_ne `{!NonExpansive sm} {i} :
-    NonExpansive (inv_sem sm i).
-  Proof. solve_proper. Qed.
+  Local Lemma inv_sem_ne {sm} :
+    □ (∀ Px Qx, Px ≡ Qx -∗ sm Px -∗ sm Qx) ⊢
+      □ (∀ i Px Qx, Px ≡ Qx -∗ inv_sem sm i Px -∗ inv_sem sm i Qx).
+  Proof.
+    iIntros "#Ne !> %%% eqv [[Px i]|?]"; [|by iRight]. iLeft. iFrame "i".
+    iApply ("Ne" with "eqv Px").
+  Qed.
 
   (** World satisfaction *)
   Local Definition inv_wsat_def (sm : FML $oi Σ -d> iProp Σ) : iProp Σ :=
@@ -69,8 +72,6 @@ Section inv.
   Qed.
   #[export] Instance inv_wsat_proper : Proper ((≡) ==> (≡)) inv_wsat.
   Proof. apply ne_proper, _. Qed.
-
-  Context `{sm : !Sem (FML $oi Σ) (iProp Σ), !NonExpansive sm}.
 
   (** Allocate [ownD] *)
   Lemma alloc_ownD (I : gset positive) N :
@@ -107,8 +108,8 @@ Section inv.
   Qed.
 
   (** Allocate [inv_tok] *)
-  Lemma inv_tok_alloc_rec Px N :
-    (inv_tok N Px -∗ ⟦ Px ⟧) =[inv_wsat ⟦⟧]=∗ inv_tok N Px.
+  Lemma inv_tok_alloc_rec {sm} Px N :
+    (inv_tok N Px -∗ sm Px) =[inv_wsat sm]=∗ inv_tok N Px.
   Proof.
     rewrite inv_tok_unseal inv_wsat_unseal. iIntros "→Px W".
     iDestruct (sinv_itok_alloc Px with "W") as (I) "big".
@@ -116,15 +117,15 @@ Section inv.
     iModIntro. iSplitL; [|iExists _; by iSplit]. iApply "→W". iLeft.
     iSplitR "D"; [|done]. iApply "→Px". iExists _; by iSplit.
   Qed.
-  Lemma inv_tok_alloc Px N : ⟦ Px ⟧ =[inv_wsat ⟦⟧]=∗ inv_tok N Px.
+  Lemma inv_tok_alloc {sm} Px N : sm Px =[inv_wsat sm]=∗ inv_tok N Px.
   Proof.
     iIntros "Px W". iApply (inv_tok_alloc_rec with "[Px] W"). by iIntros.
   Qed.
 
   (** Allocate [inv_tok] before storing the content *)
-  Lemma inv_tok_alloc_open {E} Px N : ↑N ⊆ E →
-    ⊢ |=[inv_wsat ⟦⟧]{E, E∖↑N}=> inv_tok N Px ∗
-      (⟦ Px ⟧ =[inv_wsat ⟦⟧]{E∖↑N, E}=∗ True).
+  Lemma inv_tok_alloc_open {sm E} Px N : ↑N ⊆ E →
+    ⊢ |=[inv_wsat sm]{E, E∖↑N}=> inv_tok N Px ∗
+      (sm Px =[inv_wsat sm]{E∖↑N, E}=∗ True).
   Proof.
     rewrite inv_tok_unseal inv_wsat_unseal=> NE. iIntros "W".
     iDestruct (sinv_itok_alloc Px with "W") as (I) "big".
@@ -140,9 +141,9 @@ Section inv.
   Qed.
 
   (** Access using [inv_tok] *)
-  Lemma inv_tok_acc {N E Px} : ↑N ⊆ E →
-    inv_tok N Px =[inv_wsat ⟦⟧]{E,E∖↑N}=∗
-      ⟦ Px ⟧ ∗ (⟦ Px ⟧ =[inv_wsat ⟦⟧]{E∖↑N,E}=∗ True).
+  Lemma inv_tok_acc {sm N E Px} : ↑N ⊆ E →
+    inv_tok N Px =[inv_wsat sm]{E,E∖↑N}=∗
+      sm Px ∗ (sm Px =[inv_wsat sm]{E∖↑N,E}=∗ True).
   Proof.
     rewrite inv_tok_unseal inv_wsat_unseal=> NE. iIntros "[%i[%iN #sm]] W".
     iMod (fupd_ownE_acc_in iN NE) as "[i cl]".
@@ -156,9 +157,9 @@ Section inv.
     iLeft. iFrame.
   Qed.
   (** Access using [inv_tok] via view shift *)
-  Lemma inv_tok_acc_vs {N Px E Q R} : ↑N ⊆ E →
-    □ (⟦ Px ⟧ -∗ Q =[inv_wsat ⟦⟧]{E∖↑N}=∗ ⟦ Px ⟧ ∗ R) -∗
-    □ (inv_tok N Px -∗ Q =[inv_wsat ⟦⟧]{E}=∗ R).
+  Lemma inv_tok_acc_vs {sm N Px E Q R} : ↑N ⊆ E →
+    □ (sm Px -∗ Q =[inv_wsat sm]{E∖↑N}=∗ sm Px ∗ R) -∗
+    □ (inv_tok N Px -∗ Q =[inv_wsat sm]{E}=∗ R).
   Proof.
     iIntros (?) "#vs !> i Q". iMod (inv_tok_acc with "i") as "[Px cl]"; [done|].
     iMod ("vs" with "Px Q") as "[Px $]". by iApply "cl".
@@ -167,13 +168,13 @@ End inv.
 
 Section inv_wp.
   Context `{!inv'GS FML Σ, !iris'GS_gen hlc Λ Σ}.
-  Context `{sm : !Sem (FML $oi Σ) (iProp Σ), !NonExpansive sm}.
 
   (** Access using [inv_tok] via [twp] *)
-  Lemma inv_tok_acc_twp `{!Atomic (stuckness_to_atomicity s) e} {N Px E Q Ψ} :
+  Lemma inv_tok_acc_twp `{!Atomic (stuckness_to_atomicity s) e}
+    {sm N Px E Q Ψ} :
     ↑N ⊆ E → to_val e = None →
-    [[{ ⟦ Px ⟧ ∗ Q }]][inv_wsat ⟦⟧] e @ s; E∖↑N [[{ v, RET v; ⟦ Px ⟧ ∗ Ψ v }]] -∗
-      [[{ inv_tok N Px ∗ Q }]][inv_wsat ⟦⟧] e @ s; E [[{ v, RET v; Ψ v }]].
+    [[{ sm Px ∗ Q }]][inv_wsat sm] e @ s; E∖↑N [[{ v, RET v; sm Px ∗ Ψ v }]] -∗
+      [[{ inv_tok N Px ∗ Q }]][inv_wsat sm] e @ s; E [[{ v, RET v; Ψ v }]].
   Proof.
     iIntros (??) "#twp %Φ !> [i Q] →Φ".
     iMod (inv_tok_acc with "i") as "[Px cl]"; [done..|].
@@ -184,8 +185,9 @@ End inv_wp.
 
 (** Allocate [inv_wsat] *)
 Lemma inv_wsat_alloc `{!inv'GpreS FML Σ, !invGS_gen hlc Σ} :
-  ⊢ |==> ∃ _ : inv'GS FML Σ, ∀ sm, inv_wsat sm.
+  ⊢ |==> ∃ _ : inv'GS FML Σ,
+    ∀ sm, □ (∀ Px Qx, Px ≡ Qx -∗ sm Px -∗ sm Qx) -∗ inv_wsat sm.
 Proof.
-  iMod sinv_wsat_alloc as (?) "W". iModIntro. iExists _. iIntros (?).
-  rewrite inv_wsat_unseal. iApply "W".
+  iMod sinv_wsat_alloc as (?) "W". iModIntro. iExists _. iIntros (?) "Ne".
+  rewrite inv_wsat_unseal. iApply "W". by iApply inv_sem_ne.
 Qed.
