nola/iris/pborrow.v
@@ -4,8 +4,8 @@ From nola.bi Require Export plist.
 From nola.bi Require Import order.
 From nola.iris Require Export borrow proph_ag.
 From iris.proofmode Require Import proofmode.
-Import ProdNotation PlistNotation SemNotation iPropAppNotation LftNotation
-  ProphNotation UpdwNotation.
+Import ProdNotation PlistNotation iPropAppNotation LftNotation ProphNotation
+  UpdwNotation.
 
 Implicit Type (TY : synty) (FML : oFunctor) (α : lft) (q : Qp).
 
@@ -192,14 +192,6 @@ Section pborrow.
   Definition plend_body_var sm {X} (ξ : prvar X) (Φx : X -d> FML $oi Σ)
     : iProp Σ := plend_body sm (λ π, π ξ) Φx.
 
-  (** [plend_body] is non-expansive *)
-  #[export] Instance plend_body_ne `{!NonExpansive sm} {X xπ} :
-    NonExpansive (@plend_body sm X xπ).
-  Proof. solve_proper. Qed.
-  #[export] Instance plend_body_var_ne `{!NonExpansive sm} {X ξ} :
-    NonExpansive (@plend_body_var sm X ξ).
-  Proof. exact _. Qed.
-
   (** Semantics of [pborrow_fml] *)
   Local Definition pbsem sm : _ -d> iProp Σ := λ Pb, match Pb with
     | xjust Px => sm Px
@@ -210,18 +202,27 @@ Section pborrow.
     end%I.
 
   (** [pbsem] is non-expansive *)
-  Local Instance pbsem_sem_ne `{!NonExpansive sm} :
-    NonExpansive (pbsem sm).
-  Proof.
-    move=> ???[_ _[_ _[|]|]|]; [solve_proper|..].
-    - move=> [?[??]][?[??]][/=?]. subst. move=>/= [/=/leibniz_equiv_iff ??].
-      solve_proper.
-    - move=> [?[??]][?[??]][/=?]. subst. move=>/= [/=/leibniz_equiv_iff ??].
-      solve_proper.
-    - move=> ?? /leibniz_equiv_iff. solve_proper.
-  Qed.
   Local Instance pbsem_ne : NonExpansive pbsem.
   Proof. move=> ????[[[?|[?[??]]]|[?[??]]]|?]//=; solve_proper. Qed.
+  (** [pbsem sm] is non-expansive if [sm] is *)
+  Local Lemma pbsem_sem_ne {sm} :
+    □ (∀ Px Qx, Px ≡ Qx -∗ sm Px -∗ sm Qx) ⊢
+      □ (∀ Pb Pb', Pb ≡ Pb' -∗ pbsem sm Pb -∗ pbsem sm Pb').
+  Proof.
+    iIntros "#Ne !>" ([s|?][s'|?]) "eqv"; rewrite sum_equivI //=; last first.
+    { iDestruct "eqv" as "<-". iIntros "$". }
+    rewrite sum_equivI; case: s=> [s|[?[??]]]; case: s'=> [s'|[?[??]]]//=;
+      last first.
+    { rewrite sigT_equivI /=. iDestruct "eqv" as (?) "eqv". subst=>/=.
+      rewrite prod_equivI /= discrete_fun_equivI.
+      iDestruct "eqv" as "[<- #eqv]". iIntros "[%[$ Φx]]".
+      by iApply ("Ne" with "[] Φx"). }
+    rewrite sum_equivI; case: s=> [?|[?[??]]]; case: s'=> [?|[?[??]]]//=.
+    { iApply ("Ne" with "eqv"). }
+    rewrite sigT_equivI /=. iDestruct "eqv" as (?) "eqv". subst=>/=.
+    rewrite prod_equivI /= discrete_fun_equivI. iDestruct "eqv" as "[<- #eqv]".
+    iIntros "[%[$ Φx]]". by iApply ("Ne" with "[] Φx").
+  Qed.
 
   (** World satisfaction *)
   Definition pborrow_wsat M sm : iProp Σ := borrow_wsat M (pbsem sm).
@@ -235,15 +236,13 @@ Section pborrow.
     Mono (OT:=_ → _ : bi) (OT':=_ → _ : bi) pborrow_wsat.
   Proof. move=> ????. by apply: borrow_wsat_mono. Qed.
 
-  Context `{sm : !Sem (FML $oi Σ) (iProp Σ), !NonExpansive sm}.
-
   (** ** For non-prophetic borrowing *)
 
   (** Create new borrowers and lenders *)
-  Lemma nbor_nlend_tok_new_list α Pxl Qxl :
-    ([∗ list] Px ∈ Pxl, ⟦ Px ⟧) -∗
-    ([†α] -∗ ([∗ list] Px ∈ Pxl, ⟦ Px ⟧) -∗ M
-      ([∗ list] Qx ∈ Qxl, ⟦ Qx ⟧)%I) =[pborrow_wsat M ⟦⟧]=∗
+  Lemma nbor_nlend_tok_new_list {sm} α Pxl Qxl :
+    ([∗ list] Px ∈ Pxl, sm Px) -∗
+    ([†α] -∗ ([∗ list] Px ∈ Pxl, sm Px) -∗ M
+      ([∗ list] Qx ∈ Qxl, sm Qx)%I) =[pborrow_wsat M sm]=∗
       ([∗ list] Px ∈ Pxl, nbor_tok α Px) ∗ [∗ list] Qx ∈ Qxl, nlend_tok α Qx.
   Proof.
     iIntros "Pxl →Qxl".
@@ -251,17 +250,17 @@ Section pborrow.
       (xjustf <$> Pxl) (xjustf <$> Qxl) with "[Pxl] [→Qxl]");
       by rewrite !big_sepL_fmap.
   Qed.
-  Lemma nbor_nlend_tok_new α Px :
-    ⟦ Px ⟧ =[pborrow_wsat M ⟦⟧]=∗ nbor_tok α Px ∗ nlend_tok α Px.
+  Lemma nbor_nlend_tok_new {sm} α Px :
+    sm Px =[pborrow_wsat M sm]=∗ nbor_tok α Px ∗ nlend_tok α Px.
   Proof.
     iIntros "Px". iMod (nbor_nlend_tok_new_list α [Px] [Px] with "[Px] []")
       as "[[$_][$_]]"; by [iFrame|iIntros|].
   Qed.
 
   (** Split a lender *)
-  Lemma nlend_tok_split {α Px} Qxl :
-    nlend_tok α Px -∗ (⟦ Px ⟧ -∗ M ([∗ list] Qx ∈ Qxl, ⟦ Qx ⟧))
-      =[pborrow_wsat M ⟦⟧]=∗ [∗ list] Qx ∈ Qxl, nlend_tok α Qx.
+  Lemma nlend_tok_split {sm α Px} Qxl :
+    nlend_tok α Px -∗ (sm Px -∗ M ([∗ list] Qx ∈ Qxl, sm Qx))
+      =[pborrow_wsat M sm]=∗ [∗ list] Qx ∈ Qxl, nlend_tok α Qx.
   Proof.
     iIntros "l →Qxl".
     iMod (lend_tok_split (M:=M) (sm:=pbsem _) (xjustf <$> Qxl)
@@ -269,21 +268,21 @@ Section pborrow.
   Qed.
 
   (** Retrieve from a lender *)
-  Lemma nlend_tok_retrieve {α Px} :
-    [†α] -∗ nlend_tok α Px -∗ modw M (pborrow_wsat M ⟦⟧) ⟦ Px ⟧.
+  Lemma nlend_tok_retrieve {sm α Px} :
+    [†α] -∗ nlend_tok α Px -∗ modw M (pborrow_wsat M sm) (sm Px).
   Proof. exact lend_tok_retrieve. Qed.
 
   (** Open a borrower *)
-  Lemma nbor_tok_open {α q Px} :
-    q.[α] -∗ nbor_tok α Px -∗ modw M (pborrow_wsat M ⟦⟧)
-      (nobor_tok α q Px ∗ ⟦ Px ⟧).
+  Lemma nbor_tok_open {sm α q Px} :
+    q.[α] -∗ nbor_tok α Px -∗ modw M (pborrow_wsat M sm)
+      (nobor_tok α q Px ∗ sm Px).
   Proof. exact bor_tok_open. Qed.
 
   (** Merge and subdivide/reborrow borrowers *)
-  Lemma nobor_tok_merge_subdiv αqPxl Qxl β :
+  Lemma nobor_tok_merge_subdiv {sm} αqPxl Qxl β :
     ([∗ list] '(α, q, Px)' ∈ αqPxl, β ⊑□ α ∗ nobor_tok α q Px) -∗
-    ([∗ list] Qx ∈ Qxl, ⟦ Qx ⟧) -∗ ([†β] -∗ ([∗ list] Qx ∈ Qxl, ⟦ Qx ⟧) -∗ M
-      ([∗ list] '(_, _, Px)' ∈ αqPxl, ⟦ Px ⟧)%I) =[pborrow_wsat M ⟦⟧]=∗
+    ([∗ list] Qx ∈ Qxl, sm Qx) -∗ ([†β] -∗ ([∗ list] Qx ∈ Qxl, sm Qx) -∗ M
+      ([∗ list] '(_, _, Px)' ∈ αqPxl, sm Px)%I) =[pborrow_wsat M sm]=∗
       ([∗ list] '(α, q, Px)' ∈ αqPxl, q.[α] ∗ ([†β] -∗ nbor_tok α Px)) ∗
       [∗ list] Qx ∈ Qxl, nbor_tok β Qx.
   Proof.
@@ -293,10 +292,10 @@ Section pborrow.
       with "[ol] [Qxl] [→Pxl]"); by rewrite !big_sepL_fmap /=.
   Qed.
   (** Subdivide/reborrow a borrower *)
-  Lemma nobor_tok_subdiv {α q Px} Qxl β :
-    β ⊑□ α -∗ nobor_tok α q Px -∗ ([∗ list] Qx ∈ Qxl, ⟦ Qx ⟧) -∗
-    ([†β] -∗ ([∗ list] Qx ∈ Qxl, ⟦ Qx ⟧) -∗ M ⟦ Px ⟧)
-      =[pborrow_wsat M ⟦⟧]=∗
+  Lemma nobor_tok_subdiv {sm α q Px} Qxl β :
+    β ⊑□ α -∗ nobor_tok α q Px -∗ ([∗ list] Qx ∈ Qxl, sm Qx) -∗
+    ([†β] -∗ ([∗ list] Qx ∈ Qxl, sm Qx) -∗ M (sm Px))
+      =[pborrow_wsat M sm]=∗
       q.[α] ∗ ([†β] -∗ nbor_tok α Px) ∗ [∗ list] Qx ∈ Qxl, nbor_tok β Qx.
   Proof.
     iIntros "⊑ o Qxl →Px".
@@ -305,24 +304,24 @@ Section pborrow.
   Qed.
 
   (** Reborrow a borrower *)
-  Lemma nobor_tok_reborrow {α q Px} β :
-    β ⊑□ α -∗ nobor_tok α q Px -∗ ⟦ Px ⟧ =[pborrow_wsat M ⟦⟧]=∗
+  Lemma nobor_tok_reborrow {sm α q Px} β :
+    β ⊑□ α -∗ nobor_tok α q Px -∗ sm Px =[pborrow_wsat M sm]=∗
       q.[α] ∗ ([†β] -∗ nbor_tok α Px) ∗ nbor_tok β Px.
   Proof.
     iIntros "⊑ o Px".
     iMod (nobor_tok_subdiv [Px] with "⊑ o [Px] []") as "($ & $ & $ & _)"=>/=;
       by [iFrame|iIntros "_ [$ _]"|].
   Qed.
-  Lemma nbor_tok_reborrow {α q Px} β :
-    β ⊑□ α -∗ q.[α] -∗ nbor_tok α Px -∗ modw M (pborrow_wsat M ⟦⟧)
+  Lemma nbor_tok_reborrow {sm α q Px} β :
+    β ⊑□ α -∗ q.[α] -∗ nbor_tok α Px -∗ modw M (pborrow_wsat M sm)
       (q.[α] ∗ ([†β] -∗ nbor_tok α Px) ∗ nbor_tok β Px).
   Proof.
     iIntros "⊑ α b". iMod (nbor_tok_open with "α b") as "[o Px]".
     by iMod (nobor_tok_reborrow with "⊑ o Px").
   Qed.
   (** Simply close a borrower *)
-  Lemma nobor_tok_close {α q Px} :
-    nobor_tok α q Px -∗ ⟦ Px ⟧ =[pborrow_wsat M ⟦⟧]=∗ q.[α] ∗ nbor_tok α Px.
+  Lemma nobor_tok_close {sm α q Px} :
+    nobor_tok α q Px -∗ sm Px =[pborrow_wsat M sm]=∗ q.[α] ∗ nbor_tok α Px.
   Proof.
     iIntros "o Px".
     iMod (nobor_tok_reborrow with "[] o Px") as "($ & _ & $)";
@@ -339,11 +338,11 @@ Section pborrow.
   Local Definition plend_list {Xl} (xπΦxl : plist (λ X, _ *' (X → _)) Xl)
     : list (pborrow_fml TY FML $oi Σ) :=
     of_plist (λ _ '(xπ, Φx)', xplend _ xπ Φx) xπΦxl.
-  Local Lemma vo_pbor_alloc_list {Xl ξl} {xΦxl : plist _ Xl} :
-    1:∗[of_plist_prvar ξl] -∗ ([∗ plist] '(x, Φx)' ∈ xΦxl, ⟦⟧ (Φx x)) ==∗ ∃ γl,
+  Local Lemma vo_pbor_alloc_list {sm Xl ξl} {xΦxl : plist _ Xl} :
+    1:∗[of_plist_prvar ξl] -∗ ([∗ plist] '(x, Φx)' ∈ xΦxl, sm (Φx x)) ==∗ ∃ γl,
       let γξxΦxl := plist_zip γl (plist_zip ξl xΦxl) in
       ([∗ plist] '(γ, _, x, _)' ∈ γξxΦxl, val_obs γ x) ∗
-      ([∗ list] Pb ∈ pbor_list γξxΦxl, pbsem ⟦⟧ Pb).
+      ([∗ list] Pb ∈ pbor_list γξxΦxl, pbsem sm Pb).
   Proof.
     elim: Xl ξl xΦxl=>/=; [iIntros; by iExists ()|].
     move=> X Xl IH [ξ ξl] [[x Φx] xΦxl]. iIntros "[ξ ξl] [Φx Φxl]".
@@ -353,22 +352,22 @@ Section pborrow.
   Qed.
 
   (** Lemma for [pbor_plend_tok_new_list] *)
-  Local Lemma pbor_list_sem_to_plend {Xl γl} {ξxΦxl : plist _ Xl} :
-    ([∗ list] Pb ∈ pbor_list (plist_zip γl ξxΦxl), pbsem ⟦⟧ Pb) ==∗
-      [∗ plist] '(ξ, _, Φx)' ∈ ξxΦxl, plend_body_var ⟦⟧ ξ Φx.
+  Local Lemma pbor_list_sem_to_plend {sm Xl γl} {ξxΦxl : plist _ Xl} :
+    ([∗ list] Pb ∈ pbor_list (plist_zip γl ξxΦxl), pbsem sm Pb) ==∗
+      [∗ plist] '(ξ, _, Φx)' ∈ ξxΦxl, plend_body_var sm ξ Φx.
   Proof.
     elim: Xl γl ξxΦxl=>/=; [by iIntros|]=> X Xl IH [γ γl] [[ξ[x Φx]] ξxΦxl].
     iIntros "[[%[pc Φx]] pborl]". iMod (IH with "pborl") as "$".
     iMod (pc_resolve with "pc") as "?". iModIntro. iExists _. iFrame.
   Qed.
   (** Create new prophetic borrowers and lenders *)
-  Lemma pbor_plend_tok_new_list Xl α (xΦxl : plist _ Xl) :
+  Lemma pbor_plend_tok_new_list {sm} Xl α (xΦxl : plist _ Xl) :
     ⊢ |==> ∃ ξl, ∀ Yl (yπΨxl : plist (λ Y, _ *' (Y → _)) Yl),
       let ξxΦxl := plist_zip ξl xΦxl in
-      ([∗ plist] '(x, Φx)' ∈ xΦxl, ⟦⟧ (Φx x)) -∗
-      ([†α] -∗ ([∗ plist] '(ξ, _, Φx)' ∈ ξxΦxl, plend_body_var ⟦⟧ ξ Φx) -∗
-        M ([∗ plist] '(yπ, Ψx)' ∈ yπΨxl, plend_body ⟦⟧ yπ Ψx))
-        =[pborrow_wsat M ⟦⟧]=∗
+      ([∗ plist] '(x, Φx)' ∈ xΦxl, sm (Φx x)) -∗
+      ([†α] -∗ ([∗ plist] '(ξ, _, Φx)' ∈ ξxΦxl, plend_body_var sm ξ Φx) -∗
+        M ([∗ plist] '(yπ, Ψx)' ∈ yπΨxl, plend_body sm yπ Ψx))
+        =[pborrow_wsat M sm]=∗
         ([∗ plist] '(ξ, x, Φx)' ∈ ξxΦxl, pbor_tok α x ξ Φx) ∗
         ([∗ plist] '(yπ, Ψx)' ∈ yπΨxl, plend_tok α yπ Ψx).
   Proof.
@@ -388,8 +387,8 @@ Section pborrow.
     rewrite pbor_tok_unseal. iRight. iExists _. iFrame.
   Qed.
   (** Simply create a prophetic borrower and a prophetic lender *)
-  Lemma pbor_plend_tok_new X α x Φx :
-    ⟦⟧ (Φx x) =[pborrow_wsat M ⟦⟧]=∗ ∃ ξ,
+  Lemma pbor_plend_tok_new {sm} X α x Φx :
+    sm (Φx x) =[pborrow_wsat M sm]=∗ ∃ ξ,
       pbor_tok (X:=X) α x ξ Φx ∗ plend_tok α (λ π, π ξ) Φx.
   Proof.
     iIntros "Φx".
@@ -400,11 +399,12 @@ Section pborrow.
   Qed.
 
   (** Split a prophetic lender *)
-  Lemma plend_tok_split {X α xπ Φx} Yl (yπΨxl : plist (λ Y, _ *' (Y → _)) Yl) :
+  Lemma plend_tok_split {sm X α xπ Φx} Yl
+    (yπΨxl : plist (λ Y, _ *' (Y → _)) Yl) :
     plend_tok (X:=X) α xπ Φx -∗
-    (plend_body ⟦⟧ xπ Φx -∗
-      M ([∗ plist] '(yπ, Ψx)' ∈ yπΨxl, plend_body ⟦⟧ yπ Ψx))
-      =[pborrow_wsat M ⟦⟧]=∗ [∗ plist] '(yπ, Ψx)' ∈ yπΨxl, plend_tok α yπ Ψx.
+    (plend_body sm xπ Φx -∗
+      M ([∗ plist] '(yπ, Ψx)' ∈ yπΨxl, plend_body sm yπ Ψx))
+      =[pborrow_wsat M sm]=∗ [∗ plist] '(yπ, Ψx)' ∈ yπΨxl, plend_tok α yπ Ψx.
   Proof.
     iIntros "/=l →Ψxl".
     iMod (lend_tok_split (M:=M) (sm:=pbsem _) (plend_list yπΨxl)
@@ -412,15 +412,15 @@ Section pborrow.
   Qed.
 
   (** Retrieve from a prophetic lender *)
-  Lemma plend_tok_retrieve {X α xπ Φx} :
-    [†α] -∗ plend_tok (X:=X) α xπ Φx -∗ modw M (pborrow_wsat M ⟦⟧)
-      (plend_body ⟦⟧ xπ Φx).
+  Lemma plend_tok_retrieve {sm X α xπ Φx} :
+    [†α] -∗ plend_tok (X:=X) α xπ Φx -∗ modw M (pborrow_wsat M sm)
+      (plend_body sm xπ Φx).
   Proof. exact: lend_tok_retrieve. Qed.
 
   (** Open a prophetic borrower *)
-  Lemma pbor_tok_open {X α q x ξ Φx} :
-    q.[α] -∗ pbor_tok (X:=X) α x ξ Φx -∗ modw M (pborrow_wsat M ⟦⟧)
-      (pobor_tok α q ξ Φx ∗ ⟦⟧ (Φx x)).
+  Lemma pbor_tok_open {sm X α q x ξ Φx} :
+    q.[α] -∗ pbor_tok (X:=X) α x ξ Φx -∗ modw M (pborrow_wsat M sm)
+      (pobor_tok α q ξ Φx ∗ sm (Φx x)).
   Proof.
     rewrite pbor_tok_unseal pobor_tok_unseal. iIntros "α [†|[%[vo b]]]".
     { iDestruct (lft_live_dead with "α †") as %[]. }
@@ -455,10 +455,10 @@ Section pborrow.
     iIntros (yl') "#obs". iDestruct ("→pcl" with "obs") as "$". iApply "→pc".
     by iApply (proph_obs_impl with "obs")=> ? ->.
   Qed.
-  Local Lemma pbor_list_sem_to_obs_sem {Yl γl' ηl} {yΨxl : plist _ Yl} :
-    ([∗ list] Qb ∈ pbor_list (plist_zip γl' (plist_zip ηl yΨxl)), pbsem ⟦⟧ Qb)
+  Local Lemma pbor_list_sem_to_obs_sem {sm Yl γl' ηl} {yΨxl : plist _ Yl} :
+    ([∗ list] Qb ∈ pbor_list (plist_zip γl' (plist_zip ηl yΨxl)), pbsem sm Qb)
       ==∗ ∃ yl', ⟨π, app_plist_prvar π ηl = yl'⟩ ∗
-      [∗ plist] '(y', _, Ψx)' ∈ plist_zip yl' yΨxl, ⟦⟧ (Ψx y').
+      [∗ plist] '(y', _, Ψx)' ∈ plist_zip yl' yΨxl, sm (Ψx y').
   Proof.
     elim: Yl γl' ηl yΨxl=>/=.
     { iIntros (_ [] _ _) "!>". iExists (). iSplit; [|done].
@@ -469,15 +469,15 @@ Section pborrow.
     iModIntro. by iApply (proph_obs_impl2 with "obs obs'")=>/= ? <- <-.
   Qed.
   (** Merge and subdivide prophetic borrowers *)
-  Lemma pobor_tok_merge_subdiv Xl Yl
+  Lemma pobor_tok_merge_subdiv {sm} Xl Yl
     (αqξΦxfl : plist (λ X, _ *' _ *' _ *' _ *' (_ → X)) Xl) (yΨxl : plist _ Yl)
     Rxl β :
     ([∗ plist] '(α, q, ξ, Φx, _)' ∈ αqξΦxfl, β ⊑□ α ∗ pobor_tok α q ξ Φx) -∗
-    ([∗ plist] '(y, Ψx)' ∈ yΨxl, ⟦ Ψx y ⟧) -∗ ([∗ list] Rx ∈ Rxl, ⟦ Rx ⟧) -∗
+    ([∗ plist] '(y, Ψx)' ∈ yΨxl, sm (Ψx y)) -∗ ([∗ list] Rx ∈ Rxl, sm Rx) -∗
     (∀ yl', [†β] -∗
-      ([∗ plist] '(y', _, Ψx)' ∈ plist_zip yl' yΨxl, ⟦ Ψx y' ⟧) -∗
-      ([∗ list] Rx ∈ Rxl, ⟦ Rx ⟧) -∗ M
-        ([∗ plist] '(_, _, _, Φx, f)' ∈ αqξΦxfl, ⟦ Φx (f yl') ⟧))
+      ([∗ plist] '(y', _, Ψx)' ∈ plist_zip yl' yΨxl, sm (Ψx y')) -∗
+      ([∗ list] Rx ∈ Rxl, sm Rx) -∗ M
+        ([∗ plist] '(_, _, _, Φx, f)' ∈ αqξΦxfl, sm (Φx (f yl'))))
       =[pborrow_wsat M sm]=∗ ∃ ηl,
       ([∗ plist] '(α, q, _)' ∈ αqξΦxfl, q.[α]) ∗
       ([∗ plist] '(_, _, ξ, _, f)' ∈ αqξΦxfl,
@@ -511,12 +511,13 @@ Section pborrow.
     rewrite pbor_tok_unseal. iRight. iExists _. iFrame.
   Qed.
   (** Subdivide a prophetic borrower *)
-  Lemma pobor_tok_subdiv {X α q ξ Φx} Yl (f : _ → X) (yΨxl : plist _ Yl) Rxl β :
-    β ⊑□ α -∗ pobor_tok α q ξ Φx -∗ ([∗ plist] '(y, Ψx)' ∈ yΨxl, ⟦ Ψx y ⟧) -∗
-    ([∗ list] Rx ∈ Rxl, ⟦ Rx ⟧) -∗
+  Lemma pobor_tok_subdiv {sm X α q ξ Φx} Yl (f : _ → X) (yΨxl : plist _ Yl) Rxl
+    β :
+    β ⊑□ α -∗ pobor_tok α q ξ Φx -∗ ([∗ plist] '(y, Ψx)' ∈ yΨxl, sm (Ψx y)) -∗
+    ([∗ list] Rx ∈ Rxl, sm Rx) -∗
     (∀ yl', [†β] -∗
-      ([∗ plist] '(y', _, Ψx)' ∈ plist_zip yl' yΨxl, ⟦ Ψx y' ⟧) -∗
-      ([∗ list] Rx ∈ Rxl, ⟦ Rx ⟧) -∗ M ⟦ Φx (f yl') ⟧)
+      ([∗ plist] '(y', _, Ψx)' ∈ plist_zip yl' yΨxl, sm (Ψx y')) -∗
+      ([∗ list] Rx ∈ Rxl, sm Rx) -∗ M (sm (Φx (f yl'))))
       =[pborrow_wsat M sm]=∗ ∃ ηl,
       q.[α] ∗ ⟨π, π (Aprvar _ ξ) = f (app_plist_prvar π ηl)⟩ ∗
       ([∗ plist] '(η, y, Ψx)' ∈ plist_zip ηl yΨxl, pbor_tok β y η Ψx) ∗
@@ -530,8 +531,8 @@ Section pborrow.
   Qed.
 
   (** Resolve the prophecy of a prophetic borrower *)
-  Lemma pobor_tok_resolve {X α q ξ Φx} x :
-    pobor_tok (X:=X) α q ξ Φx -∗ ⟦ Φx x ⟧ =[pborrow_wsat M sm]=∗
+  Lemma pobor_tok_resolve {sm X α q ξ Φx} x :
+    pobor_tok (X:=X) α q ξ Φx -∗ sm (Φx x) =[pborrow_wsat M sm]=∗
       q.[α] ∗ ⟨π, π ξ = x⟩ ∗ nbor_tok α (Φx x).
   Proof.
     iIntros "o Φx".
@@ -539,7 +540,7 @@ Section pborrow.
       as (?) "[$[$[_[$ _]]]]"=>/=;
       by [iApply lft_sincl_refl|iFrame|iIntros "% _ _ [$ _]"|].
   Qed.
-  Lemma pbor_tok_resolve {X α q x ξ Φx} :
+  Lemma pbor_tok_resolve {sm X α q x ξ Φx} :
     q.[α] -∗ pbor_tok (X:=X) α x ξ Φx -∗ modw M (pborrow_wsat M sm)
       (q.[α] ∗ ⟨π, π ξ = x⟩ ∗ nbor_tok α (Φx x)).
   Proof.
@@ -548,9 +549,9 @@ Section pborrow.
   Qed.
 
   (** Subdivide a prophetic borrower without changing the prophecy *)
-  Lemma pobor_tok_nsubdiv {X α q ξ Φx} Ψx x β :
-    β ⊑□ α -∗ pobor_tok (X:=X) α q ξ Φx -∗ ⟦ Ψx x ⟧ -∗
-    (∀ x', [†β] -∗ ⟦ Ψx x' ⟧ -∗ M ⟦ Φx x' ⟧) =[pborrow_wsat M sm]=∗
+  Lemma pobor_tok_nsubdiv {sm X α q ξ Φx} Ψx x β :
+    β ⊑□ α -∗ pobor_tok (X:=X) α q ξ Φx -∗ sm (Ψx x) -∗
+    (∀ x', [†β] -∗ sm (Ψx x') -∗ M (sm (Φx x'))) =[pborrow_wsat M sm]=∗
       q.[α] ∗ pbor_tok β x ξ Ψx.
   Proof.
     rewrite pobor_tok_unseal pbor_tok_unseal.
@@ -564,8 +565,8 @@ Section pborrow.
     iModIntro. iRight. iExists _. iFrame.
   Qed.
   (** Simply close a prophetic borrower *)
-  Lemma pobor_tok_close {X α q ξ Φx} x :
-    pobor_tok (X:=X) α q ξ Φx -∗ ⟦ Φx x ⟧ =[pborrow_wsat M sm]=∗
+  Lemma pobor_tok_close {sm X α q ξ Φx} x :
+    pobor_tok (X:=X) α q ξ Φx -∗ sm (Φx x) =[pborrow_wsat M sm]=∗
       q.[α] ∗ pbor_tok α x ξ Φx.
   Proof.
     iIntros "o Φx". iApply (pobor_tok_nsubdiv Φx with "[] o Φx"); [|by iIntros].
@@ -573,9 +574,9 @@ Section pborrow.
   Qed.
 
   (** Reborrow a nested prophetic borrower *)
-  Lemma pobor_pobor_tok_reborrow {X Y α q ξ Φx β r η Ψx} y f : β ⊑□ α -∗
-    pobor_tok (X:=X) β q ξ Φx -∗ pobor_tok (X:=Y) α r η Ψx -∗ ⟦ Ψx y ⟧ -∗
-    (∀ y', [†β] -∗ pbor_tok α y' η Ψx -∗ M ⟦ Φx (f y') ⟧) -∗
+  Lemma pobor_pobor_tok_reborrow {sm X Y α q ξ Φx β r η Ψx} y f : β ⊑□ α -∗
+    pobor_tok (X:=X) β q ξ Φx -∗ pobor_tok (X:=Y) α r η Ψx -∗ sm (Ψx y) -∗
+    (∀ y', [†β] -∗ pbor_tok α y' η Ψx -∗ M (sm (Φx (f y')))) -∗
       modw M (pborrow_wsat M sm) (∃ η' : prvar _,
       q.[β] ∗ r.[α] ∗ ⟨π, π ξ = f (π η')⟩ ∗ pbor_tok β y η' Ψx).
   Proof.
@@ -616,9 +617,9 @@ Section pborrow.
     iApply modw_fold. iModIntro. rewrite pbor_tok_unseal. iRight. iExists _.
     iFrame.
   Qed.
-  Lemma pobor_pbor_tok_reborrow {X Y α q ξ Φx β r y η Ψx} f : β ⊑□ α -∗
+  Lemma pobor_pbor_tok_reborrow {sm X Y α q ξ Φx β r y η Ψx} f : β ⊑□ α -∗
     pobor_tok (X:=X) β q ξ Φx -∗ r.[α] -∗ pbor_tok (X:=Y) α y η Ψx -∗
-    (∀ y', [†β] -∗ pbor_tok α y' η Ψx -∗ M ⟦ Φx (f y') ⟧) -∗
+    (∀ y', [†β] -∗ pbor_tok α y' η Ψx -∗ M (sm (Φx (f y')))) -∗
       modw M (pborrow_wsat M sm) (∃ η' : prvar _,
       q.[β] ∗ r.[α] ∗ ⟨π, π ξ = f (π η')⟩ ∗ pbor_tok β y η' Ψx).
   Proof.
@@ -629,8 +630,10 @@ End pborrow.
 
 (** Allocate [pborrow_wsat] *)
 Lemma pborrow_wsat_alloc `{!pborrowGpreS TY FML Σ} :
-  ⊢ |==> ∃ _ : pborrowGS TY FML Σ, ∀ M sm, pborrow_wsat M sm.
+  ⊢ |==> ∃ _ : pborrowGS TY FML Σ,
+    ∀ M sm, □ (∀ Px Qx, Px ≡ Qx -∗ sm Px -∗ sm Qx) -∗ pborrow_wsat M sm.
 Proof.
-  iMod proph_init as (?) "_". iMod borrow_wsat_alloc as (?) "?".
-  iModIntro. iExists (PborrowGS _ _ _ _ _ _). by iIntros.
+  iMod proph_init as (?) "_". iMod borrow_wsat_alloc as (?) "big".
+  iModIntro. iExists (PborrowGS _ _ _ _ _ _). iIntros (??) "Ne". iApply "big".
+  by iApply pbsem_sem_ne.
 Qed.
